wip

code/api/Hacl.AEAD.Chacha20Poly1305.fst
@@ -1,12 +1,16 @@
 module Hacl.AEAD.Chacha20Poly1305
 
+open FStar.Seq
 open FStar.HyperStack
 open FStar.Buffer
 open FStar.ST
 open Hacl.Constants
 open Hacl.Policies
 open Hacl.Cast
+open Hacl.Spec.Endianness
 open Hacl.Endianness
+
+open Spec.Chacha20Poly1305
 
 (* Module abbreviations *)
 
@@ -18,6 +22,7 @@ module U64 = FStar.UInt64
 module H8  = Hacl.UInt8
 module H32 = Hacl.UInt32
 module H64 = Hacl.UInt64
+
 
 (* The following values should point to Spec.Chacha20Poly1305 *)
 let noncelen = 12
@@ -48,6 +53,44 @@ private let lemma_aead_encrypt_poly h0 h1 h2 h3 h4 r acc mac =
 
 
 #reset-options "--initial_fuel 0 --max_fuel 0 --z3rlimit 50"
+open FStar.Mul
+
+assume val lemma_encode_bytes_append: s1:Seq.seq U8.t -> s2:Seq.seq U8.t -> l:nat{l * 16 = Seq.length s1} ->
+  Lemma (requires (True))
+        (ensures (Spec.Poly1305.encode_bytes (s1 @| s2) == Spec.Poly1305.encode_bytes s2 @| Spec.Poly1305.encode_bytes s1))
+        (* (decreases (l)) *)
+
+assume private val encode_bytes_append: len:nat -> s:Seq.seq U8.t -> w:Spec.Poly1305.word -> Lemma
+  (requires (0 < Seq.length w /\ Seq.length s == len /\ len % 16 == 0))
+  (ensures  (Seq.equal (Spec.Poly1305.encode_bytes ((Seq.append s w)))
+                      (Seq.cons (w) (Spec.Poly1305.encode_bytes (s)))))
+
+open FStar.Endianness 
+
+private val lemma_aead_encrypt_poly_2:
+  k:Spec.Poly1305.key ->
+  mac:Spec.Poly1305.tag ->
+  aad:Seq.seq H8.t ->
+  c:Seq.seq H8.t ->
+  lb:Spec.Poly1305.word_16 ->
+  Lemma (requires (
+    let r = Spec.Poly1305.encode_r (slice k 0 16) in
+    let s = hlittle_endian (slice k 16 32) in
+    hlittle_endian mac = (Spec.Poly1305.poly (Seq.cons lb (Spec.Poly1305.encode_bytes (pad_16 c) @| Spec.Poly1305.encode_bytes (pad_16 aad))) r + s) % pow2 128))
+        (ensures (mac == Spec.Poly1305.poly1305 (pad_16 aad @| pad_16 c @| lb) k))
+#reset-options "--initial_fuel 0 --max_fuel 0 --z3rlimit 100"
+let lemma_aead_encrypt_poly_2 k mac aad c lb =
+  Math.Lemmas.lemma_div_mod (Seq.length (pad_16 aad)) 16;
+  lemma_encode_bytes_append (pad_16 aad) (pad_16 c) (Seq.length (pad_16 aad) / 16);
+  cut (Spec.Poly1305.encode_bytes (pad_16 aad @| pad_16 c) == Spec.Poly1305.encode_bytes (pad_16 c) @| Spec.Poly1305.encode_bytes (pad_16 aad));
+  let s = (pad_16 aad @| pad_16 c) in
+  Seq.lemma_eq_intro (pad_16 aad @| pad_16 c @| lb) ((pad_16 aad @| pad_16 c) @| lb);
+  encode_bytes_append (Seq.length s) s lb;  
+  cut (Seq.cons lb (Spec.Poly1305.encode_bytes (pad_16 c) @| Spec.Poly1305.encode_bytes (pad_16 aad))
+    == Spec.Poly1305.encode_bytes (pad_16 aad @| pad_16 c @| lb));
+  lemma_little_endian_inj (Spec.Poly1305.poly1305 (pad_16 aad @| pad_16 c @| lb) k) mac
+
+
 
 private val aead_encrypt_poly:
   c:uint8_p ->
@@ -55,14 +98,20 @@ private val aead_encrypt_poly:
   mac:uint8_p{length mac = maclen /\ disjoint mac c} ->
   aad:uint8_p ->
   aadlen:u32{let len = U32.v aadlen in len = length aad}  ->
-  k:uint8_p{length k = keylen /\ disjoint k mac} ->
-  n:uint8_p{length n = noncelen /\ disjoint n mac} ->
   b:uint8_p{length b >= 80 /\ disjoint b mac} ->
   Stack unit
-    (requires (fun h -> live h c /\ live h mac /\ live h n /\ live h k /\ live h aad /\ live h b))
-    (ensures  (fun h0 z h1 -> modifies_1 mac h0 h1 /\ live h1 mac))
-#reset-options "--initial_fuel 0 --max_fuel 0 --z3rlimit 100"
-private let aead_encrypt_poly  c mlen mac aad aadlen k n tmp =
+    (requires (fun h -> live h c /\ live h mac /\ live h aad /\ live h b))
+    (ensures  (fun h0 z h1 -> live h0 c /\ live h0 mac /\ live h0 aad /\ live h0 b
+      /\ modifies_1 mac h0 h1 /\ live h1 mac
+      /\ (let k   = reveal_sbytes (as_seq h0 (Buffer.sub b 0ul 32ul)) in
+         let aad = reveal_sbytes (as_seq h0 aad) in
+         let c   = reveal_sbytes (as_seq h0 c) in
+         let mac = reveal_sbytes (as_seq h1 mac) in
+         let lb  = reveal_sbytes (as_seq h0 (Buffer.sub b 64ul 16ul)) in
+         mac == Spec.Poly1305.poly1305 (pad_16 aad @| pad_16 c @| lb) k)
+    ))
+#reset-options "--initial_fuel 0 --max_fuel 0 --z3rlimit 200"
+private let aead_encrypt_poly  c mlen mac aad aadlen tmp =
   let b = Buffer.sub tmp 0ul 64ul in
   let lb = Buffer.sub tmp 64ul 16ul in
   let mk = Buffer.sub b 0ul 32ul in
@@ -71,14 +120,32 @@ private let aead_encrypt_poly  c mlen mac aad aadlen k n tmp =
   let h0 = ST.get() in
   let tmp = Buffer.create (uint64_to_sint64 0uL) 6ul in
   let st = Poly1305_64.mk_state (Buffer.sub tmp 0ul 3ul) (Buffer.sub tmp 3ul 3ul) in
-  (* let st = Poly1305_64.alloc () in *)
   let h1 = ST.get() in
   let log:log_t = Poly1305_64.poly1305_blocks_init st aad aadlen mk in
   let h2 = ST.get() in
+  cut (let aad = as_seq h0 aad in
+       let r   = Spec.Poly1305.encode_r (as_seq h0 (Buffer.sub mk 0ul 16ul)) in
+       let acc = Hacl.Spec.Poly1305_64.selem (as_seq h2 Hacl.Impl.Poly1305_64.(st.h)) in
+       acc     = Spec.Poly1305.poly (Spec.Poly1305.encode_bytes (pad_16 aad)) r);
   let log:log_t = Poly1305_64.poly1305_blocks_continue log st c mlen in
   let h3 = ST.get() in
+  cut (let aad = as_seq h0 aad in
+       let r   = Spec.Poly1305.encode_r (as_seq h0 (Buffer.sub mk 0ul 16ul)) in
+       let acc = Hacl.Spec.Poly1305_64.selem (as_seq h3 Hacl.Impl.Poly1305_64.(st.h)) in
+       let c   = reveal_sbytes (as_seq h0 c) in
+       acc     = Spec.Poly1305.poly (Spec.Poly1305.encode_bytes (pad_16 c) @| Spec.Poly1305.encode_bytes (pad_16 aad)) r);
   Poly1305_64.poly1305_blocks_finish log st lb mac key_s;
   let h4 = ST.get() in
+  cut (let lb  = as_seq h0 lb in
+       let c   = as_seq h0 c in
+       let aad = as_seq h0 aad in
+       let r   = Spec.Poly1305.encode_r (as_seq h0 (Buffer.sub mk 0ul 16ul)) in
+       let s   = hlittle_endian (as_seq h0 (Buffer.sub mk 16ul 16ul)) in
+       let mac = reveal_sbytes (as_seq h4 mac) in
+       hlittle_endian mac = (Spec.Poly1305.poly (Seq.cons lb (Spec.Poly1305.encode_bytes (pad_16 c) @| Spec.Poly1305.encode_bytes (pad_16 aad))) r + s) % pow2 128);
+  Seq.lemma_eq_intro (as_seq h0 (Buffer.sub mk 0ul 16ul)) (Seq.slice (as_seq h0 mk) 0 16);
+  Seq.lemma_eq_intro (as_seq h0 (Buffer.sub mk 16ul 16ul)) (Seq.slice (as_seq h0 mk) 16 32);
+  lemma_aead_encrypt_poly_2 (as_seq h0 mk) (as_seq h4 mac) (as_seq h0 aad) (as_seq h0 c) (as_seq h0 lb);
   lemma_aead_encrypt_poly h0 h1 h2 h3 h4 Hacl.Impl.Poly1305_64.(st.r) Hacl.Impl.Poly1305_64.(st.h) mac;
   pop_frame()
 
@@ -124,6 +191,9 @@ let aead_encrypt c mac m mlen aad aadlen k n =
   hstore64_le (Buffer.sub lb 0ul 8ul) (uint32_to_sint64 aadlen);
   hstore64_le (Buffer.sub lb 8ul 8ul) (uint32_to_sint64 mlen);
   let h1 = ST.get() in
+  Seq.lemma_eq_intro (as_seq h1 b) (as_seq h1 (Buffer.sub lb 0ul 8ul) @| as_seq h1 (Buffer.sub lb 8ul 8ul)); admit()
+  cut (as_seq h1 lb == little_bytes 8ul (length aad) @| little_bytes 8ul (length c));
+  admit()
   cut (modifies_0 h0 h1);
   Chacha20.chacha20 c m mlen k n 1ul;
   let h2 = ST.get() in
