code/poly1305/interfaces/Poly1305_64.fsti
@@ -131,59 +131,61 @@ val poly1305_blocks_init:
          let acc = as_seq h1 I.(st.h) in
          let log = reveal log in
          let m   = reveal_sbytes (as_seq h0 input) in
+         let kr  = reveal_sbytes (as_seq h0 (Buffer.sub k 0ul 16ul)) in
          Hacl.Spe.Poly1305_64.invariant (MkState r acc log)
+         /\ Hacl.Spec.Poly1305_64.seval r = Spec.Poly1305.encode_r kr
          /\ log == Spec.Poly1305.encode_bytes (pad_16 m))
     ))
 
 
-(* val poly1305_blocks_continue: *)
-(*   log:I.log_t -> *)
-(*   st:I.poly1305_state -> *)
-(*   input:uint8_p{disjoint I.(st.h) input} -> *)
-(*   len:U32.t{U32.v len = length input} -> *)
-(*   Stack I.log_t *)
-(*     (requires (fun h -> I.live_st h st /\ live h input *)
-(*       /\ (let r = as_seq h I.(st.r) in *)
-(*          let acc = as_seq h I.(st.h) in *)
-(*          let log = reveal log in *)
-(*          Hacl.Spe.Poly1305_64.invariant (Hacl.Spec.Poly1305_64.MkState r acc log)) *)
-(*     )) *)
-(*     (ensures (fun h0 log' h1 -> I.live_st h0 st /\ I.live_st h1 st /\ live h0 input *)
-(*       /\ modifies_1 I.(st.h) h0 h1 *)
-(*       /\ (let r = as_seq h0 I.(st.r) in *)
-(*          let acc = as_seq h0 I.(st.h) in *)
-(*          let log = reveal log in *)
-(*          let acc' = as_seq h1 I.(st.h) in *)
-(*          let log' = reveal log' in *)
-(*          let m    = reveal_sbytes (as_seq h0 input) in *)
-(*          Hacl.Spe.Poly1305_64.invariant (Hacl.Spec.Poly1305_64.MkState r acc log) *)
-(*          /\ Hacl.Spe.Poly1305_64.invariant (Hacl.Spec.Poly1305_64.MkState r acc' log') *)
-(*          /\ log' == Seq.append (Spec.Poly1305.encode_bytes (pad_16 m)) log) *)
-(*     )) *)
+val poly1305_blocks_continue:
+  log:I.log_t ->
+  st:I.poly1305_state ->
+  input:uint8_p{disjoint I.(st.h) input} ->
+  len:U32.t{U32.v len = length input} ->
+  Stack I.log_t
+    (requires (fun h -> I.live_st h st /\ live h input
+      /\ (let r = as_seq h I.(st.r) in
+         let acc = as_seq h I.(st.h) in
+         let log = reveal log in
+         Hacl.Spe.Poly1305_64.invariant (Hacl.Spec.Poly1305_64.MkState r acc log))
+    ))
+    (ensures (fun h0 log' h1 -> I.live_st h0 st /\ I.live_st h1 st /\ live h0 input
+      /\ modifies_1 I.(st.h) h0 h1
+      /\ (let r = as_seq h0 I.(st.r) in
+         let acc = as_seq h0 I.(st.h) in
+         let log = reveal log in
+         let acc' = as_seq h1 I.(st.h) in
+         let log' = reveal log' in
+         let m    = reveal_sbytes (as_seq h0 input) in
+         Hacl.Spe.Poly1305_64.invariant (Hacl.Spec.Poly1305_64.MkState r acc log)
+         /\ Hacl.Spe.Poly1305_64.invariant (Hacl.Spec.Poly1305_64.MkState r acc' log')
+         /\ log' == Seq.append (Spec.Poly1305.encode_bytes (pad_16 m)) log)
+    ))
 
 
-(* val poly1305_blocks_finish: *)
-(*   log:I.log_t -> *)
-(*   st:I.poly1305_state -> *)
-(*   input:uint8_p{disjoint I.(st.h) input /\ length input = 16} -> *)
-(*   mac:uint8_p{disjoint I.(st.h) mac /\ disjoint mac input /\ length mac = 16} -> *)
-(*   key_s:uint8_p{disjoint key_s I.(st.h) /\ disjoint key_s mac /\ length key_s = 16} -> *)
-(*   Stack unit *)
-(*     (requires (fun h -> I.live_st h st /\ live h input /\ live h mac /\ live h key_s *)
-(*       /\ (let r = as_seq h I.(st.r) in *)
-(*          let acc = as_seq h I.(st.h) in *)
-(*          let log = reveal log in *)
-(*          Hacl.Spe.Poly1305_64.invariant (Hacl.Spec.Poly1305_64.MkState r acc log)) *)
-(*     )) *)
-(*     (ensures (fun h0 _ h1 -> I.live_st h0 st /\ live h0 key_s /\ live h0 input *)
-(*       /\ modifies_2 mac I.(st.h) h0 h1 /\ live h1 mac *)
-(*       /\ (let mac = as_seq h1 mac in *)
-(*          let r   = (as_seq h0 I.(st.r)) in *)
-(*          let acc = as_seq h0 I.(st.h) in *)
-(*          let log = reveal log in *)
-(*          let m   = reveal_sbytes (as_seq h0 input) in *)
-(*          let k   = Hacl.Spec.Endianness.hlittle_endian (as_seq h0 key_s) in *)
-(*          Hacl.Spe.Poly1305_64.invariant (Hacl.Spec.Poly1305_64.MkState r acc log) *)
-(*          /\ Hacl.Spec.Endianness.hlittle_endian mac *)
-(*            == (Spec.Poly1305.poly (Seq.cons m log) (Hacl.Spec.Bignum.Bigint.seval r) + k) % pow2 128) *)
-(*     )) *)
+val poly1305_blocks_finish:
+  log:I.log_t ->
+  st:I.poly1305_state ->
+  input:uint8_p{disjoint I.(st.h) input /\ length input = 16} ->
+  mac:uint8_p{disjoint I.(st.h) mac /\ disjoint mac input /\ length mac = 16} ->
+  key_s:uint8_p{disjoint key_s I.(st.h) /\ disjoint key_s mac /\ length key_s = 16} ->
+  Stack unit
+    (requires (fun h -> I.live_st h st /\ live h input /\ live h mac /\ live h key_s
+      /\ (let r = as_seq h I.(st.r) in
+         let acc = as_seq h I.(st.h) in
+         let log = reveal log in
+         Hacl.Spe.Poly1305_64.invariant (Hacl.Spec.Poly1305_64.MkState r acc log))
+    ))
+    (ensures (fun h0 _ h1 -> I.live_st h0 st /\ live h0 key_s /\ live h0 input
+      /\ modifies_2 mac I.(st.h) h0 h1 /\ live h1 mac
+      /\ (let mac = as_seq h1 mac in
+         let r   = (as_seq h0 I.(st.r)) in
+         let acc = as_seq h0 I.(st.h) in
+         let log = reveal log in
+         let m   = reveal_sbytes (as_seq h0 input) in
+         let k   = Hacl.Spec.Endianness.hlittle_endian (as_seq h0 key_s) in
+         Hacl.Spe.Poly1305_64.invariant (Hacl.Spec.Poly1305_64.MkState r acc log)
+         /\ Hacl.Spec.Endianness.hlittle_endian mac
+           == (Spec.Poly1305.poly (Seq.cons m log) (seval r) + k) % pow2 128)
+    ))
